Cslib/Languages/LambdaCalculus/LocallyNameless/Untyped/StrongNorm.lean
@@ -7,6 +7,7 @@ Authors: David Wegmann
 module
 
 public import Cslib.Languages.LambdaCalculus.LocallyNameless.Untyped.FullBeta
+public import Cslib.Languages.LambdaCalculus.LocallyNameless.Untyped.FullEta
 public import Cslib.Languages.LambdaCalculus.LocallyNameless.Untyped.MultiApp
 public import Cslib.Languages.LambdaCalculus.LocallyNameless.Untyped.LcAt
 public import Cslib.Foundations.Relation.Confluence
@@ -155,6 +156,92 @@ lemma sn_abs_app_multiApp [DecidableEq Var] [HasFresh Var] {Ps} {M N : Term Var}
               right
               refine Relation.TransGen.single (Xi.base (Beta.beta ?_ ?_))
               all_goals grind
+
+lemma sn_abs_rev [DecidableEq Var] [HasFresh Var] (M : Term Var) (x : Var)
+  (hx : x ∉ M.fv) (sn_M_abs : SN FullBeta M.abs) :
+  SN FullBeta (M ^ (fvar x)) := by
+  generalize h : M.abs = M_open at sn_M_abs
+  induction sn_M_abs generalizing M with
+  | intro MM h ih =>
+      constructor
+      intro z h_step
+      subst MM
+      have z_lc : LC z := step_lc_r h_step
+      rw [<- close_open x z 0 z_lc] at h_step
+      have g := @step_abs_close _ _ _ _ _ x h_step
+      rw [close_openRec_to_subst _ _ _ _ z_lc (LC.fvar _), subst_refl] at g
+      unfold open' at g
+      rw [<- open_close _ _ _ hx] at g
+      specialize ih _ g (z⟦0 ↜ x⟧) (by grind) (by rfl)
+      unfold open' at ih
+      rw [close_openRec_to_subst _ _ _ _ z_lc (LC.fvar _), subst_refl] at ih
+      assumption
+
+
+-- trival
+lemma sn_app_rev (t s : Term Var) (h : SN FullBeta (t.app s)) :
+     ∀ {t' s' : Term Var}, t ↠βᶠ t'.abs → s ↠βᶠ s' → SN FullBeta (t' ^ s') := by
+  intros t' s' h_t_red h_s_red
+  sorry
+
+lemma foo [DecidableEq Var] [HasFresh Var] (Z M N : Term Var) (h : FullEta M N)
+  (g : ∀ {t s : Term Var}, Z ↠βᶠ t.abs → M ↠βᶠ s → SN FullBeta (t ^ s)) :
+       ∀ {t s : Term Var}, Z ↠βᶠ t.abs → N ↠βᶠ s → SN FullBeta (t ^ s) := by
+  sorry
+
+-- based on baz
+-- and postpone eta-step (proved)
+lemma bar [DecidableEq Var] [HasFresh Var] (Z M N : Term Var) (h : FullEta M N)
+  (g : ∀ {t s : Term Var}, M ↠βᶠ t.abs → Z ↠βᶠ s → SN FullBeta (t ^ s)) :
+       ∀ {t s : Term Var}, N ↠βᶠ t.abs → Z ↠βᶠ s → SN FullBeta (t ^ s) := by
+  sorry
+
+lemma baz [DecidableEq Var] [HasFresh Var] (s : Term Var) (s_lc : s.LC)
+  (t_st_t' : t.abs ⭢ηᶠ t'.abs) (sn_t : SN FullBeta (t ^ s)) : SN FullBeta (t' ^ s) := by
+  cases t_st_t' with
+  | base t_st_t' => cases t_st_t' with
+                    | eta t'_lc =>  unfold open' at sn_t
+                                    unfold openRec at sn_t
+                                    rw [open_lc _ _ _ t'_lc] at sn_t
+                                    exact sn_step (Xi.base (Beta.beta t'_lc s_lc)) sn_t
+  | abs xs ih => sorry
+
+lemma sn_eta_step [DecidableEq Var] [HasFresh Var]
+  (t_st_t' : t ⭢ηᶠ t') (sn_t : SN FullBeta t) : SN FullBeta t' := by
+  induction t_st_t' with
+  | base h => cases h
+              have ⟨x, _⟩ := fresh_exists <| free_union [fv] Var
+              have g := sn_abs_rev _ x (by grind) sn_t
+              unfold open' at g
+              unfold openRec at g
+              apply sn_app_left at g
+              · rw [open_lc] at g <;> assumption
+              · apply LC.fvar
+  | appL _ _ ih =>  rename_i Z M N _ _
+                    apply sn_app
+                    · apply sn_app_left
+                      pick_goal 2
+                      · exact sn_t
+                      apply FullEta.step_lc_l
+                      assumption
+                    · apply ih
+                      apply sn_app_right <;> assumption
+                    · clear ih
+                      sorry
+  | appR _ _ ih =>  apply sn_app
+                    · apply ih
+                      · apply sn_app_left
+                        pick_goal 2
+                        · exact sn_t
+                        assumption
+                    · apply sn_app_right
+                      pick_goal 2
+                      · exact sn_t
+                      apply FullEta.step_lc_l
+                      assumption
+                    · sorry
+  | abs xs _ ih =>  have ⟨x, _⟩ := fresh_exists <| free_union [fv] Var
+                    exact sn_abs (ih x (by grind) (sn_abs_rev _ x (by grind) sn_t)) (LC.fvar x)
 
 end LambdaCalculus.LocallyNameless.Untyped.Term
 
